

# 1 Diffusion Equations and Parabolic Problems

## 1.1 Stability Analysis

Note the Fourier transform of a function  $v(x)$  is defined as

$$\hat{v}(k) = \frac{1}{\sqrt{2\pi}} \int_{-\infty}^{\infty} v(x) e^{-ikx} dx. \quad (1)$$

The inverse Fourier transform is given by

$$v(x) = \frac{1}{\sqrt{2\pi}} \int_{-\infty}^{\infty} \hat{v}(k) e^{ikx} dk. \quad (2)$$

We first note  $\hat{v}(k)$  is also called the Fourier coefficient of  $v(x)$  for wave number  $k$ . We also note for any real  $kx$  that  $e^{ikx} = \cos(kx) + i \sin(kx)$  by Euler's formula.

### 1.1.1 Differentiation and Fourier Transform

We can derive

$$\frac{d}{dx} v(x) = \frac{1}{\sqrt{2\pi}} \int_{-\infty}^{\infty} i k \hat{v}(k) e^{ikx} dk \quad (3)$$

And we call the  $ik$  term in the integrand above the *symbol* of the differential operator  $d/dx$ .

We also note, for a function of two variables  $u(x, t)$ , the Fourier transform of

spatial variable  $x$  is given by

$$\hat{u}(k, t) = \frac{1}{\sqrt{2\pi}} \int_{-\infty}^{\infty} u(x, t) e^{-ikx} dx, \quad (4)$$

and its inverse is given by

$$u(x, t) = \frac{1}{\sqrt{2\pi}} \int_{-\infty}^{\infty} \hat{u}(k, t) e^{ikx} dk. \quad (5)$$

Now we can try to look at the advection equation

$$\frac{\partial u}{\partial t} = -c \frac{\partial u}{\partial x}, \quad u(x, 0) = \eta(x). \quad (6)$$

Note the Fourier transform for  $u$  w.r.t.  $x$  is  $\hat{u} = \frac{1}{\sqrt{2\pi}} \int_{-\infty}^{\infty} u(x, t) e^{-ikx} dx$ , and we can see

$$\frac{\partial}{\partial t} \frac{1}{\sqrt{2\pi}} \int_{-\infty}^{\infty} \hat{u}(k, t) e^{ikx} dk = -c \frac{\partial u}{\partial x} \frac{1}{\sqrt{2\pi}} \int_{-\infty}^{\infty} \hat{u}(k, t) e^{ikx} dk \quad (7)$$

This is equivalent to the following

$$\int_{-\infty}^{\infty} \frac{\partial \hat{u}(k, t)}{\partial t} e^{ikx} dk = -c \int_{-\infty}^{\infty} \frac{\partial}{\partial x} (\hat{u}(k, t) e^{ikx}) dk = -c \int_{-\infty}^{\infty} ik \hat{u}(k, t) e^{ikx} dk \quad (8)$$

As we have the equality of the integrands, we can write the ODE for  $\hat{u}(k, t)$

as

$$\frac{\partial \hat{u}(k, t)}{\partial t} = -cik\hat{u}(k, t). \quad (9)$$

This is a first order ODE in  $t$  and we can solve it to get

$$\hat{u}(k, t) = \hat{u}(k, 0)e^{-cikt} = \hat{\eta}(k)e^{-cikt}. \quad (10)$$

We also should note that the Fourier transform of the initial condition is given by  $\hat{u}(k, 0) = \frac{1}{\sqrt{2\pi}} \int_{-\infty}^{\infty} \eta(x)e^{-ikx}dx = \hat{\eta}(k)$ . We can now take the inverse Fourier transform of the above (10) to get

$$u(x, t) = \frac{1}{\sqrt{2\pi}} \int_{-\infty}^{\infty} \hat{u}(k, 0)e^{-cikt}e^{ikx}dk \quad (11)$$

This is equivalent to

$$u(x, t) = \frac{1}{\sqrt{2\pi}} \int_{-\infty}^{\infty} \hat{u}(k, 0)e^{ik(x-ct)}dk = \frac{1}{\sqrt{2\pi}} \int_{-\infty}^{\infty} \hat{\eta}(k)e^{ik(x-ct)}dk \quad (12)$$

Using change of variables  $x - ct = x'$ , we can write

$$u(x, t) = \frac{1}{\sqrt{2\pi}} \int_{-\infty}^{\infty} \hat{\eta}(k)e^{ikx'}dk = \eta(x - ct). \quad (13)$$

This is the solution to the advection equation, which means the solution is advected at a speed  $c$  from the initial condition  $\eta(x)$ .

Note from (10) that the solution is stable if  $|e^{-cikt}| = 1$ .

**Note for 1d diffusion equation (infinite spatial domain):**

$$\frac{\partial u}{\partial t} = \alpha \frac{\partial^2 u}{\partial x^2}, \quad u(x, 0) = \eta(x). \quad (14)$$

We can take the Fourier transform of the above equation to get

$$\frac{\partial \hat{u}(k, t)}{\partial t} = -\alpha k^2 \hat{u}(k, t). \quad (15)$$

This is a first order ODE in  $t$  and we can solve it to get

$$\hat{u}(k, t) = \hat{u}(k, 0)e^{-\alpha k^2 t} = \hat{\eta}(k)e^{-\alpha k^2 t}. \quad (16)$$

Obviously this means

$$|\hat{u}(k, t)| = |\hat{\eta}(k)|e^{-\alpha k^2 t}. \quad (17)$$

So in diffusion equation, the Fourier coefficient of the solution decays exponentially in time

### 1.1.2 Symbol for difference operators

Now we will check the *symbols* of difference operators in the finite difference method.

If  $x$  is shifted by  $\Delta x$  then we can see

$$\begin{aligned} u(x + \Delta x) &= \frac{1}{\sqrt{2\pi}} \int_{-\infty}^{\infty} \hat{u}(k) e^{ik(x+\Delta x)} dk \\ &= \frac{1}{\sqrt{2\pi}} \int_{-\infty}^{\infty} e^{ik\Delta x} \hat{u}(k) e^{ikx} dk \end{aligned} \quad (18)$$

Suppose  $d/dx$  is approximated by the central difference operator

$$\begin{aligned} D_0 u(x) &= \frac{u(x + \Delta x) - u(x - \Delta x)}{2\Delta x} \\ &= \frac{1}{\sqrt{2\pi}} \int_{-\infty}^{\infty} \hat{u}(k) e^{ikx} \left( \frac{e^{ik\Delta x} - e^{-ik\Delta x}}{2\Delta x} \right) dk \\ &= \frac{1}{\sqrt{2\pi}} \int_{-\infty}^{\infty} \hat{u}(k) e^{ikx} \frac{i \sin(k\Delta x)}{\Delta x} dk \end{aligned} \quad (19)$$

The **symbol** of the above central difference operator  $D$  is given by  $i \sin(k\Delta x)/\Delta x$ .

Now consider:

$$\begin{aligned} \frac{i \sin(k\Delta x)}{\Delta x} &= \frac{i}{\Delta x} \left( k\Delta x - \frac{(k\Delta x)^3}{3!} + \frac{(k\Delta x)^5}{5!} - \dots \right) \\ &= ik - \frac{ik^3\Delta x^2}{3!} + \frac{ik^5\Delta x^4}{5!} - \dots \\ &= ik \left( 1 - \frac{k^2\Delta x^2}{3!} + \frac{k^4\Delta x^4}{5!} - \dots \right) \end{aligned} \quad (20)$$

We can see the difference between the symbol of the central difference operator and the symbol of the exact differential operator is given by  $O(\Delta x^2)$ , if  $k\Delta x$  is small enough ( $k\Delta x < 1$ ). In other word, it means  $k$  is considerably smaller than  $1/\Delta x = N$ .

We note

$$\begin{aligned}
\frac{\partial^2 u}{\partial x^2} &= \frac{\partial}{\partial x} \left( \frac{\partial u}{\partial x} \right) \\
&= \frac{\partial}{\partial x} \left( \frac{1}{\sqrt{2\pi}} \int_{-\infty}^{\infty} \hat{u}(k) e^{ikx} dk \right) \\
&= \frac{1}{\sqrt{2\pi}} \int_{-\infty}^{\infty} \hat{u}(k) \frac{\partial}{\partial x} e^{ikx} dk \\
&= \frac{1}{\sqrt{2\pi}} \int_{-\infty}^{\infty} \hat{u}(k) (ik) e^{ikx} dk \\
&= \frac{1}{\sqrt{2\pi}} \int_{-\infty}^{\infty} (ik)^2 \hat{u}(k) e^{ikx} dk \\
&= -k^2 \hat{u}(k).
\end{aligned} \tag{21}$$

The **symbol** of the central difference operator for the second derivative is given by  $-k^2$ .

Now consider the central difference operator for second derivative.

$$\begin{aligned}
D_0 u(x) &= \frac{u(x + \Delta x) - 2u(x) + u(x - \Delta x)}{\Delta x^2} \\
&= \frac{1}{\sqrt{2\pi}} \int_{-\infty}^{\infty} \hat{u}(k) e^{ikx} \left( \frac{e^{ik\Delta x} - 2 + e^{-ik\Delta x}}{\Delta x^2} \right) dk \\
&= \frac{1}{\sqrt{2\pi}} \int_{-\infty}^{\infty} \hat{u}(k) e^{ikx} \left( \frac{2 \cos(k\Delta x) - 2}{\Delta x^2} \right) dk
\end{aligned} \tag{22}$$

$$\begin{aligned}
\frac{2 \cos(k\Delta x) - 2}{\Delta x^2} &= \frac{2}{\Delta x^2} (\cos(k\Delta x) - 1) \\
&= \frac{2}{\Delta x^2} \left( 1 - \frac{k^2 \Delta x^2}{2!} + \frac{k^4 \Delta x^4}{4!} - \dots - 1 \right) \\
&= \frac{2}{\Delta x^2} \left( -k^2 \Delta x^2 + \frac{k^4 \Delta x^4}{3!} - \dots \right) \\
&= -k^2 + \frac{k^4 \Delta x^2}{3!} - \dots
\end{aligned} \tag{23}$$

So the difference between the symbol of the central difference operator for the second derivative and the symbol of the exact differential operator is  $O(\Delta x^2)$ , given  $k$  is considerably small.

### 1.1.3 Eigengridfunction and von Neumann stability analysis

Given function in  $x$  with  $e^{ix\xi}$ , we notice

$$\frac{\partial}{\partial x} e^{ix\xi} = \partial_x e^{ix\xi} = i\xi e^{ix\xi}, \quad \partial_x^2 e^{ix\xi} = -\xi^2 e^{ix\xi}.$$

Now given grid function  $W_j = e^{ijh\xi} = e^{ij\Delta x\xi}$ , has the property of being an eigengridfunction of the translation-invariant finite difference operator:

$$W_{j+1} = e^{i(j+1)h\xi} = e^{ijh\xi} e^{ih\xi} = e^{ijh\xi} e^{i\xi} = W_j e^{i\xi}. \quad (24)$$

$$W_{j-1} = e^{i(j-1)h\xi} = e^{ijh\xi} e^{-ih\xi} = e^{ijh\xi} e^{-i\xi} = W_j e^{-i\xi}. \quad (25)$$

So we can see the finite difference operator for the first derivative has the symbol  $i\xi$ . We can also see

$$\begin{aligned} D_0 W_j &= \frac{1}{2h} (W_{j+1} - W_{j-1}) = \frac{1}{2h} (e^{i(j+1)h\xi} - e^{-i(j-1)h\xi}) \\ &= \frac{1}{2h} e^{ijh\xi} (e^{ih\xi} - e^{-ih\xi}) = \frac{i}{h} e^{ijh\xi} \sin(h\xi) = \frac{i}{h} \sin(h\xi) W_j. \end{aligned} \quad (26)$$

So  $W_j$  is an eigengridfunction of the finite difference operator  $D_0$  for the first derivative with the symbol  $i \sin(h\xi)/h$  (or we say eigenvalue).

Now consider we have grid function  $V_j$  defined at grid points  $x_j = j\Delta x = jh$ , for  $j = 0, \pm 1, \pm 2, \dots$ . We also assume  $V_j$  is  $l_2$  function which means

$$\|V\|_2 = \left( h \sum_{j=-\infty}^{\infty} |V_j|^2 \right)^{\frac{1}{2}} < \infty$$

Then we can express  $V_j$  in terms of the eigengridfunctions  $W_j$  as

$$V_j = \frac{1}{\sqrt{2\pi}} \int_{-\pi/h}^{\pi/h} \hat{V}(\xi) e^{i\xi jh} d\xi = \frac{1}{\sqrt{2\pi}} \int_{-\pi/h}^{\pi/h} \hat{V}(\xi) W_j d\xi. \quad (27)$$

with the Fourier coefficients  $\hat{V}(\xi) = \frac{h}{\sqrt{2\pi}} \sum_{j=-\infty}^{\infty} V_j e^{-i j h \xi}$ .

Parseval's relation still holds  $\|\hat{V}\|_2 = \|V\|_2$ , but using the grid norms:

$$\|V\|_2 = \left( h \sum_{j=-\infty}^{\infty} |V_j|^2 \right)^{1/2}, \quad \|\hat{V}\|_2 = \left( h \int_{-\pi/h}^{\pi/h} |\hat{V}(\xi)|^2 d\xi \right)^{1/2}.$$

Now we will discuss the von Neumann stability analysis for the finite difference method.

- It is based on the decomposition of the errors into Fourier series.
- Study growth of waves  $e^{i\xi x}$
- The method is **limited to constant coefficient linear PDEs**.
- Usually applied to the Cauchy problem (space with no boundaries  $-\infty < x < \infty$  in 1D).



- Can also be applied to periodic boundary conditions.
- Note that  $e^{i\xi x}$  are eigenfunctions of the differential operator  $\partial_x$ , where  $\xi$  is the wavenumber.

$$\frac{\partial}{\partial x} (e^{i\xi x}) =$$

- Then  $W_j = e^{ijh\xi}$ ,  $h = 1/(m+1)$ ,  $j = 1, \dots, m$  is an eigenfunction of any translation-invariant finite difference operator.

- For stability, we want to show  $\|U^{n+1}\|_2 \leq (1 + \alpha\Delta t)\|U^n\|_2$  for all  $U^n$

- From Parvesal's relation, we can show  $\|\hat{U}^{n+1}\|_2 \leq (1 + \alpha\Delta t)\|\hat{U}^n\|_2$  for all  $\hat{U}^n$

- For a one step method, we expect to obtain  $\hat{U}^{n+1}(\xi) = g(\xi)\hat{U}^n(\xi)$ 
  - $g(\xi)$  is called the **amplification factor**.
  - The necessary and sufficient condition for the error to remain bounded is that  $|g(\xi)| \leq 1$ .

### 1.1.4 Examples

Apply von Neumann stability analysis to

$$U_j^{n+1} = U_j^n + \frac{\Delta t}{\Delta x^2} (U_{j-1}^n - 2U_j^n + U_{j+1}^n). \quad (28)$$

and specify the amplification factor.

We work on a single wave number  $\xi$ , and set the  $n$  level grid function to  $U_j^n = e^{ijh\xi}$  and expect  $U_j^{n+1} = g(\xi)U_j^n = g(\xi)e^{ijh\xi}$  from the finite difference method (28). From the method in (28), we can then write

$$\begin{aligned} g(\xi)e^{ijh\xi} &= e^{ijh\xi} + \frac{\Delta t}{\Delta x^2} (e^{i(j-1)h\xi} - 2e^{ijh\xi} + e^{i(j+1)h\xi}), \\ g(\xi) &= 1 + \frac{\Delta t}{\Delta x^2} (e^{-ih\xi} - 2 + e^{ih\xi}) = 1 + 2\frac{\Delta t}{\Delta x^2} (\cos(h\xi) - 1) \end{aligned} \quad (29)$$

**Example:** Compute the amplification factor for Crank-Nicholson:

$$-rU_{j-1}^{n+1} + (1 + 2r)U_j^{n+1} - rU_{j+1}^{n+1} = rU_{j-1}^n + (1 - 2r)U_j^n + rU_{j+1}^n,$$

where  $r = \frac{\Delta t}{2\Delta x^2}$ .